\documentclass{article}

\usepackage{amsmath}
\usepackage{parskip}
\usepackage{tikz}
\renewcommand{\emph}{\textbf}
\renewcommand{\bar}{\overline}
\DeclareMathOperator{\Log}{Log}
\DeclareMathOperator{\Arg}{Arg}
\DeclareMathOperator{\sech}{sech}
\DeclareMathOperator{\csch}{csch}

\begin{document}

\section{Frame 56 -- Sequences and Series}

\textbf{3}
If
\[
	\lim_{n \to \infty} z_n = z
\]
then, for some integer $n_0$, all of the terms $z_k$ ($k > n_0$) will be in some $\epsilon$ neighbourhood of $z$; ie:
\[
	|z_k - z| < \epsilon
\]
However,
\[
	||z_k| - |z| \le \epsilon
\]
so all of the terms $|z_k|$ must be inside the same $\epsilon$ neighbourhood of $|z|$, and we can say that
\[
	\lim_{n \to \infty} |z_n| = |z|
\]

\textbf{4}
Starting from the series
\[
	\sum_{n=1}^\infty z^n = \frac{1}{1 - z} - 1 = \frac{z}{1 - z}
\]
the components of this expression can be written as
\begin{align*}
	\frac{z}{1 - z}
	&= \frac{r \cos \theta + i r \sin \theta}{1 - r \cos \theta - i r \sin \theta} \\
	&= \frac{r\cos \theta - r^2 \cos^2 \theta - r^2 \sin^2 \theta}{(1 - r\cos \theta)^2 + r^2 \sin^2 \theta}
	+ i \frac{r\sin \theta - r^2 \sin \theta \cos \theta + r^2 \sin \theta \cos \theta}{(1 - r\cos \theta)^2 + r^2 \sin^2 \theta} \\
	&= \frac{r \cos \theta - r^2}{1 - 2r\cos \theta + r^2}
	+ i\frac{r\sin \theta}{1 - 2r\cos \theta + r^2}
\end{align*}
so, equating the real and imaginary parts of the sum,
\[
	\sum_{n=1}^\infty r^n \cos n\theta
	= \frac{r \cos \theta - r^2}{1 - 2r\cos \theta + r^2}
\]
and
\[
	\sum_{n=1}^\infty r^n \sin n\theta
	= \frac{r\sin \theta}{1 - 2r\cos \theta + r^2}
\]


\clearpage
\section{Frame 59 -- Taylor Series}
\textbf{1}
The Maclaurin series for $z \cosh(z^2)$ is
\[
	z \cosh(z^2)
	= z \cdot \sum_{n=0}^\infty \frac{(z^2)^{2n}}{(2n)!}
	= \sum_{n=0}^\infty \frac{z^{4n+1}}{(2n)!}
\]

\textbf{3}
The Maclaurin series for this function is
\[
	\frac{z}{9} \frac{1}{1 + (z^4/9)}
	= \frac{z}{9} \sum_{n=0}^\infty (-1)^n (z^4/9)^n
	= \sum_{n=0}^\infty \frac{(-1)^n z^{4n+1}}{9^{n+1}}
\]

\textbf{4}
Starting with the Maclaurin series for $\sin z$, this function's expansion is
\[
	\sin(z^2)
	= \sum_{n=0}^\infty \frac{(-1)^n}{(2n+1)!} (z^2)^{2n + 1}
	= \sum_{n=0}^\infty \frac{(-1)^n}{(2n+1)!} z^{4n+2}
\]
Thus, $a_k$ is only non-zero for $k = 2, 6, 10, 14, \dots$.

\textbf{10}
The function $\tanh z$ has singularities wherever $\cosh z = 0$, which occurs at $z = (k + 1/2) \pi i$. Thus, the closest singularity has a radius of $\pi/2$, and this is the radius of convergence.

We can find some of the terms of the Taylor series. The constant is
\[
	\tanh(0) = 0
\]
The first derivative is
\[
	\frac{d}{dz} \tanh(z) \Big|_{z=0}
	= \sech^2(0)
	= 1
\]
The second derivative is
\[
	\frac{d}{dz} \sech^2(z) \Big|_{z=0}
	= 2\sech(z) \cdot (-\sech z \tanh z) \Big|_{z=0}
	= -2\sech^2 z \tanh z \Big|_{z=0}
	= 0
\]
The third derivative is
\[
	\frac{d}{dz} -2\sech^2 z \tanh z \Big|_{z=0}
	= -2 \left[ -2\sech^2 z \tanh^2 z + \sech^4 z \right] \Big|_{z=0}
	= -2
\]
so the first few terms of the Taylor series are
\[
	\tanh z \approx z - \frac{z^3}{3}
\]

\textbf{11(a)}
The series for this function is
\[
	\frac{e^z}{z^2}
	= \frac{1}{z^2} \sum_{n=0}^\infty \frac{z^n}{n!}
	= \sum_{n=0}^\infty \frac{z^{n-2}}{n!}
	= \frac{1}{z^2} + \frac{1}{z} + \sum_{n=0}^\infty \frac{z^n}{(n+2)!}
\]

\textbf{11(b)}
The series for this function is
\begin{align*}
	\frac{\sin(z^2)}{z^4}
	&= \frac{1}{z^4} \sum_{n=0}^\infty \frac{(-1)^n}{(2n+1)!} (z^2)^{2n+1} \\
	&= \sum_{n=0}^\infty \frac{(-1)^n}{(2n+1)!} z^{4n - 2} \\
	&= \frac{1}{z^2} + \sum_{n=0}^\infty \frac{(-1)^{n+1}}{(2n+3)!} z^{4n+2}
\end{align*}


\clearpage
\section{Frame 62 -- Laurent Series}
\textbf{1}
The Laurent series for this function is
\begin{align*}
	z^2 \sin\left( \frac{1}{z^2} \right)
	&= z^2 \sum_{n=0}^\infty \frac{(-1)^n}{(2n+1)!} \left( \frac{1}{z^2} \right)^{2n+1} \\
	&= \sum_{n=0}^\infty \frac{(-1)^n}{(2n+1)!} \frac{1}{z^{4n}} \\
	&= 1 + \sum_{n=1}^\infty \frac{(-1)^n}{(2n+1)!} \frac{1}{z^{4n}}
\end{align*}

\textbf{2}
The Laurent series for this function is
\begin{align*}
	\frac{e^z}{(z+1)^2}
	&= \frac{1}{(z+1)^2} \frac{e^{z+1}}{e} \\
	&= \frac{1}{e} \frac{1}{(z+1)^2} \sum_{n=0}^\infty \frac{(z+1)^n}{n!} \\
	&= \frac{1}{e} \sum_{n=0}^\infty \frac{(z+1)^{n-2}}{n!} \\
	&= \frac{1}{e} \left[ \sum_{n=0}^\infty \frac{(z+1)^n}{(n+2)!} + \frac{1}{z+1} + \frac{1}{(z+1)^2} \right]
\end{align*}

\textbf{3}
The Laurent series for this function is
\begin{align*}
	\frac{1}{1 + z}
	&= \frac{1}{z} \frac{1}{1 + 1/z} \\
	&= \frac{1}{z} \sum_{n=0}^\infty \frac{(-1)^n}{z^n} \\
	&= \sum_{n=0}^\infty \frac{(-1)^n}{z^{n+1}} \\
	&= \sum_{n=1}^\infty \frac{(-1)^{n-1}}{z^n}
\end{align*}

\textbf{6}
This function's Laurent series is
\begin{align*}
	\frac{z}{(z-1)(z-3)}
	&= \frac{(z-1) + 1}{(z-1) \cdot (z-1 - 2)} \\
	&= -\frac{1}{2} \frac{1}{1 - (z-1)/2} - \frac{1}{2} \frac{1}{(z-1) \cdot (1 - (z-1)/2} \\
	&= -\frac{1}{2} \left[ \sum_{n=0}^\infty \frac{(z-1)^n}{2^n} + \sum_{n=0}^\infty \frac{(z-1)^{n-1}}{2^n} \right] \\
	&= - \sum_{n=0}^\infty \frac{(z-1)^n}{2^{n+1}} - \sum_{n=0}^\infty \frac{(z-1)^n}{2^{n+2}} - \frac{1}{2} \frac{1}{z-1} \\
	&= -3 \sum_{n=0}^\infty \frac{(z-1)^n}{2^{n+2}} - \frac{1}{2(z-1)}
\end{align*}

\textbf{7}
In the domain $1 < |z| < \infty$, this function is
\begin{align*}
	\frac{1}{z(1 + z^2)}
	&= \frac{1}{z^3} \frac{1}{1 + 1/z^2} \\
	&= \frac{1}{z^3} \sum_{n=0}^\infty \frac{(-1)^n}{z^{2n}} \\
	&= \sum_{n=1}^\infty \frac{(-1)^{n+1}}{z^{2n+1}}
\end{align*}


\clearpage
\section{Frame 66 -- Integrating and Differentiating Power Series}
\textbf{1}
Since
\[
	\frac{d}{dz} \frac{1}{1 - z} = \frac{1}{(1 - z)^2}
\]
we can write
\begin{align*}
	\frac{1}{(1 - z)^2} 
	&= \sum_{n=0}^\infty \frac{d}{dz} z^{n} \\
	&= \sum_{n=-1}^\infty nz^{n-1} \\
	&= \sum_{n=0}^\infty (n+1)z^n
\end{align*}

\textbf{3}
The Taylor series for $1/z$ is
\begin{align*}
	\frac{1}{z}
	&= \frac{1}{2 + (z - 2)} \\
	&= \frac{1}{2} \frac{1}{1 + (z - 2)/2} \\
	&= \frac{1}{2} \sum_{n=0}^\infty (-1)^n \frac{(z - 2)^n}{2^n} \\
	&= \sum_{n=0}^\infty (-1)^n \frac{1}{2^{n+1}} (z - 2)^n
\end{align*}
Then, since $-\frac{d}{dz} \frac{1}{z} = \frac{1}{z^2}$, the series for $\frac{1}{z^2}$ is
\begin{align*}
	\frac{1}{z^2}
	&= -\sum_{n=0}^\infty \frac{(-1)^n}{2^{n+1}} \frac{d}{dz} (z - 2)^n \\
	&= -\sum_{n=0}^\infty \frac{(-1)^n}{2^{n+1}} n(z - 2)^{n-1} \\
	&= \sum_{n=0}^\infty \frac{(-1)^n}{2^{n+2}} (n+1) (z - 2)^n \\
	&= \frac{1}{4} \sum_{n=0}^\infty (-1)^n (n+1) \left( \frac{z - 2}{2} \right)^n
\end{align*}

\textbf{4}
The Maclaurin series for $\sin z / z$ is
\begin{align*}
	\frac{\sin z}{z}
	&= \frac{1}{z} \sum_{n=0}^\infty \frac{(-1)^n}{(2n + 1)!} z^{2n+1} \\
	&= \sum_{n=0}^\infty \frac{(-1)^n}{(2n + 1)!} z^{2n}
\end{align*}
Evaluating this at $z = 0$ gives
\[
	\lim_{z \to 0} \frac{\sin z}{z}
	= \sum_{n=0}^\infty \frac{(-1)^n}{(2n + 1)!} (0)^{2n}
	= 1
	= f(0)
\]
so this function is entire.

\textbf{5}
A series for 
\[
	f(z) = \frac{\cos z}{(z + \pi/2)(z - \pi/2)}
\]
centered at $z_0 = -\pi/2$ is
\begin{align*}
	f(z)
	&= \frac{1}{z + \pi/2}{z - \pi/2} \sin(z + \pi/2) \\
	&= \frac{1}{z + \pi/2}{z - \pi/2} \sum_{n=0}^\infty \frac{(-1)^n}{(2n+1)!} (z + \pi/2)^{2n+1} \\
	&= \frac{1}{z - \pi/2} \sum_{n=0}^\infty \frac{(-1)^n}{(2n+1)!} (z + \pi/2)^{2n}
\end{align*}
At $z = -\pi/2$, this is
\begin{align*}
	f(\pi/2) 
	&= \frac{1}{-\pi} \sum_{n=0}^\infty \frac{(-1)^n}{(2n+1)}! (0)^{2n} \\
	&= -\frac{1}{\pi}
\end{align*}
so the function is continuous at $z = -\pi/2$. A similar proof would work for $z = +\pi/2$.

\textbf{6}
On this limited domain,
\[
	\int_{1}^{z} \frac{1}{w} dw
	= \Log w \Big|_1^z
	= \Log z - 0
	= \Log z
\]
so
\begin{align*}
	\Log z 
	&= \sum_{n=0}^\infty \int (-1)^n (z - 1)^n \\
	&= \sum_{n=0}^\infty \frac{(-1)^n}{n+1} (z - 1)^{n+1} \\
	&= \sum_{n=1}^\infty \frac{(-1)^{n-1}}{n} (z - 1)^n 
\end{align*}

\textbf{7}
By dividing through by a factor of $z - 1$, we find that
\begin{align*}
	\frac{\Log z}{z - 1}
	&= \frac{1}{1 - z} \sum_{n=1}^\infty \frac{(-1)^{n-1}}{n} (z - 1)^n  \\
	&= \sum_{n=1}^\infty \frac{(-1)^{n-1}}{n} (z - 1)^{n-1} \\
	&= \sum_{n=0}^\infty \frac{(-1)^n}{n+1} (z - 1)^n
\end{align*}
Then, at $z = 1$, this sum is $1$, so the function is analytic at this point and throughout the specified domain.

\end{document}